proving SemanticLemmas.v

platform/cito/Dict.v
@@ -1,3 +1,5 @@
+Require Import Sets.
+
 Set Implicit Arguments.
 
 Module Type KEY.
@@ -12,35 +14,36 @@ End DATA.
 Module Dict (MKey : KEY) (MData : DATA).
 
   Import MKey MData.
+
+  Module SetKey : S with Definition A := key.
+    Definition A := key.
+    Definition eq_dec := eq_dec.
+  End SetKey.
+  Module MSet := Make SetKey.
+
   Definition map := key -> data.
 
-  Definition dict := (list key * map)%type.
+  Definition dict := (MSet.set * map)%type.
 
   Definition upd_map (m : map) k v k' :=
     if eq_dec k' k then v else m k'.
 
-  Require Import List.
+  Definition keys (d : dict) := fst d.
 
-  Definition sel (d : dict) (k : key) : option data.
-    admit.
-  Defined.
+  Definition mem (d : dict) (k : key) := fst d k.
 
-  Definition upd (d : dict) k v := ((k :: fst d), upd_map (snd d) k v).
+  Definition sel (d : dict) (k : key) := snd d k.
 
-  Definition keys (d : dict) : list key.
-    admit.
-  Defined.
+  Definition upd (d : dict) k v := (MSet.add (fst d) k, upd_map (snd d) k v).
 
-  Definition remove (d : dict) (k : key) : dict.
-    admit.
-  Defined.
+  Definition remove (d : dict) (k : key) := (MSet.del (fst d) k, snd d).
 
-  Lemma sel_upd_eq : forall m k v k', k' = k ->  sel (upd m k v) k' = Some v.
-    admit. (*intros; unfold upd; destruct (eq_dec k' k); intuition.*)
+  Lemma sel_upd_eq : forall m k v k', k' = k ->  sel (upd m k v) k' = v.
+    intros; unfold sel, upd, upd_map; simpl; destruct (eq_dec k' k); intuition.
   Qed.
 
   Lemma sel_upd_ne : forall m k v k', k' <> k -> sel (upd m k v) k' = sel m k'.
-    admit. (*intros; unfold upd; destruct (eq_dec k' k); intuition.*)
+    intros; unfold sel, upd, upd_map; simpl; destruct (eq_dec k' k); intuition.
   Qed.
 
 End Dict.
